src/Util/FisherYates/Correctness.dfy
@@ -12,38 +12,18 @@ module FisherYates.Correctness {
   import RealArith
   import Measures
   import Loops
-
-  /************
-   Definitions
-  ************/
-
-  predicate IsPermutationOf<T(==)>(p: seq<T>, s: seq<T>) {
-    && multiset(p) == multiset(s)
-    && |p| == |s|
-  }
-
-  // Calculates the number n of permutations of a sequence s
-  function NumberOfPermutationsOf<T(==)>(s: seq<T>): (n: nat)
-    ensures n != 0
-  {
-    if |s| <= 1 then
-      1
-    else
-      var multiplicity := multiset(s)[s[0]];
-      var length := |s|;
-      (length / multiplicity) * NumberOfPermutationsOf(s[1..])
-  }
+  import Permutations
 
   /*******
    Lemmas
   *******/
 
   lemma CorrectnessFisherYates<T(!new)>(xs: seq<T>, p: seq<T>)
-    requires IsPermutationOf(p, xs)
+    requires Permutations.IsPermutationOf(p, xs)
     ensures
       var e := iset s | Model.Shuffle(xs)(s).Equals(p);
       && e in Rand.eventSpace
-      && Rand.prob(e) == 1.0 / (NumberOfPermutationsOf(xs) as real)
+      && Rand.prob(e) == 1.0 / (Permutations.NumberOfPermutationsOf(xs) as real)
   {
     var e := iset s | Model.Shuffle(xs)(s).Equals(p);
     var e' := iset s | Model.Shuffle(xs, 0)(s).Result? && Model.Shuffle(xs, 0)(s).value[0..] == p[0..];
@@ -51,84 +31,85 @@ module FisherYates.Correctness {
     CorrectnessFisherYatesGeneral(xs, p, 0);
   }
 
-  lemma CorrectnessFisherYatesGeneral<T(!new)>(xs: seq<T>, p: seq<T>, i: nat)
+  lemma {:axiom} CorrectnessFisherYatesGeneral<T(!new)>(xs: seq<T>, p: seq<T>, i: nat)
     requires i <= |xs|
     requires i <= |p|
-    requires IsPermutationOf(p[i..], xs[i..])
+    requires Permutations.IsPermutationOf(p[i..], xs[i..])
     decreases |xs| - i
     ensures
       var e := iset s | Model.Shuffle(xs, i)(s).Result? && Model.Shuffle(xs, i)(s).value[i..] == p[i..];
       && e in Rand.eventSpace
-      && Rand.prob(e) == 1.0 / (NumberOfPermutationsOf(xs[i..]) as real)
-  {
-    var e := iset s | Model.Shuffle(xs, i)(s).Result? && Model.Shuffle(xs, i)(s).value[i..] == p[i..];
-    if |xs[i..]| <= 1 {
-      assert e == Measures.SampleSpace() by {
-        forall s
-          ensures s in e
-        {
-          calc {
-            s in e;
-            Model.Shuffle(xs, i)(s).Result? && Model.Shuffle(xs, i)(s).value[i..] == p[i..];
-            { assert Model.Shuffle(xs, i)(s) == Monad.Return(xs)(s); }
-            Monad.Return(xs)(s).Result? && Monad.Return(xs)(s).value[i..] == p[i..];
-            { assert Monad.Return(xs)(s).value == xs; }
-            xs[i..] == p[i..];
-            if |xs[i..]| == 0 then [] == p[i..] else [xs[i]] == p[i..];
-            { assert |xs[i..]| == |p[i..]|; }
-            if |xs[i..]| == 0 then true else [xs[i]] == [p[i]];
-            { assert multiset(p[i..]) == multiset(xs[i..]); }
-            true;
-          }
-        }
-      }
-      Rand.ProbIsProbabilityMeasure();
-      assert Measures.IsProbability(Rand.eventSpace, Rand.prob);
-    } else {
-      var h := Uniform.Model.IntervalSample(i, |xs|);
-      assert HIsIndependent: Independence.IsIndep(h) by {
-        Uniform.Correctness.IntervalSampleIsIndep(i, |xs|);
-      }
-      var multiplicity := multiset(xs[i..])[xs[i]];
-      var length := |xs[i..]|;
-      var A := iset j | i <= j < |xs| && xs[j] == p[i];
-      assert A != iset{} by {
-        assume {:axiom} false;
-        assert IsPermutationOf(p[i..], xs[i..]);
-      }
-      var j :| j in A;
-      var ys := Model.Swap(xs, i, j);
-      var e' := iset s | Model.Shuffle(ys, i+1)(s).Result? && Model.Shuffle(ys, i+1)(s).value[i+1..] == p[i+1..];
-      assume {:axiom} false;
-      /*
-    assert DecomposeE: e == (iset s | s in Monad.BitstreamsWithValueIn(h, A) && s in Monad.BitstreamsWithRestIn(h, e')) by {
-      assume {:axiom} false;
-    } 
+      && Rand.prob(e) == 1.0 / (Permutations.NumberOfPermutationsOf(xs[i..]) as real)
+  /*  {
+     Permutations.PermutationsPreserveCardinality(p[i..], xs[i..]);
+     var e := iset s | Model.Shuffle(xs, i)(s).Result? && Model.Shuffle(xs, i)(s).value[i..] == p[i..];
+     if |xs[i..]| <= 1 {
+       assert e == Measures.SampleSpace() by {
+         forall s
+           ensures s in e
+         {
            calc {
-      Rand.prob(e);
-      Rand.prob(iset s | Model.Shuffle(xs, i)(s).Result? && Model.Shuffle(xs, i)(s).value[i..] == p[i..]);
-      { reveal DecomposeE; }
-      Rand.prob(iset s | s in Monad.BitstreamsWithValueIn(h, A) && s in Monad.BitstreamsWithRestIn(h, e'));
-      { reveal HIsIndependent; Independence.ResultsIndependent(h, A, e'); }
-      Rand.prob(iset s | s in Monad.BitstreamsWithValueIn(h, A)) * Rand.prob(e');
-      { assume {:axiom} false; }
-      //{ CorrectnessMultiset(xs, p[i], i); CorrectnessFisherYatesGeneral(xs, p, i+1); }
-      (multiplicity as real / length as real) * (1.0 / (NumberOfPermutationsOf(xs[i+1..]) as real));
-      { assume {:axiom} false; }
-      (1.0 / ((length as real) / (multiplicity as real))) *  (1.0 / (NumberOfPermutationsOf(xs[i+1..]) as real));
-      { assume {:axiom} false; }
-      (1.0 / ((length / multiplicity) as real)) *  (1.0 / (NumberOfPermutationsOf(xs[i+1..]) as real));
-      { assume {:axiom} false; assert 1.0 * 1.0 == 1.0; assert ((length / multiplicity) as real) * (NumberOfPermutationsOf(xs[i+1..]) as real) == (((length / multiplicity) * NumberOfPermutationsOf(xs[i+1..])) as real); }
-      1.0 / (((length / multiplicity) * NumberOfPermutationsOf(xs[i+1..])) as real);    
-      { assume {:axiom} false; assert xs[i+1..] == xs[i..][1..]; }        
-      1.0 / (((length / multiplicity) * NumberOfPermutationsOf(xs[i..][1..])) as real);  
-      { assume {:axiom} false; }      
-      1.0 / (NumberOfPermutationsOf(xs[i..]) as real);
-    } */
-    }
-  }
+             s in e;
+             Model.Shuffle(xs, i)(s).Result? && Model.Shuffle(xs, i)(s).value[i..] == p[i..];
+             { assert Model.Shuffle(xs, i)(s) == Monad.Return(xs)(s); }
+             Monad.Return(xs)(s).Result? && Monad.Return(xs)(s).value[i..] == p[i..];
+             { assert Monad.Return(xs)(s).value == xs; }
+             xs[i..] == p[i..];
+             if |xs[i..]| == 0 then [] == p[i..] else [xs[i]] == p[i..];
+             { assert |xs[i..]| == |p[i..]|; }
+             if |xs[i..]| == 0 then true else [xs[i]] == [p[i]];
+             { assert multiset(p[i..]) == multiset(xs[i..]); }
+             true;
+           }
+         }
+       }
+       Rand.ProbIsProbabilityMeasure();
+       assert Measures.IsProbability(Rand.eventSpace, Rand.prob);
+     } else {
+       var h := Uniform.Model.IntervalSample(i, |xs|);
+       assert HIsIndependent: Independence.IsIndep(h) by {
+         Uniform.Correctness.IntervalSampleIsIndep(i, |xs|);
+       }
+       var multiplicity := multiset(xs[i..])[xs[i]];
+       var length := |xs[i..]|;
+       var A := iset j | i <= j < |xs| && xs[j] == p[i];
+       assert A != iset{} by {
+         assume {:axiom} false;
+         assert Permutations.IsPermutationOf(p[i..], xs[i..]);
+       }
+       var j :| j in A;
+       var ys := Permutations.Swap(xs, i, j);
+       var e' := iset s | Model.Shuffle(ys, i+1)(s).Result? && Model.Shuffle(ys, i+1)(s).value[i+1..] == p[i+1..];
+       assume {:axiom} false;
+       /*
+     assert DecomposeE: e == (iset s | s in Monad.BitstreamsWithValueIn(h, A) && s in Monad.BitstreamsWithRestIn(h, e')) by {
+       assume {:axiom} false;
+     } 
+            calc {
+       Rand.prob(e);
+       Rand.prob(iset s | Model.Shuffle(xs, i)(s).Result? && Model.Shuffle(xs, i)(s).value[i..] == p[i..]);
+       { reveal DecomposeE; }
+       Rand.prob(iset s | s in Monad.BitstreamsWithValueIn(h, A) && s in Monad.BitstreamsWithRestIn(h, e'));
+       { reveal HIsIndependent; Independence.ResultsIndependent(h, A, e'); }
+       Rand.prob(iset s | s in Monad.BitstreamsWithValueIn(h, A)) * Rand.prob(e');
+       { assume {:axiom} false; }
+       //{ CorrectnessMultiset(xs, p[i], i); CorrectnessFisherYatesGeneral(xs, p, i+1); }
+       (multiplicity as real / length as real) * (1.0 / (NumberOfPermutationsOf(xs[i+1..]) as real));
+       { assume {:axiom} false; }
+       (1.0 / ((length as real) / (multiplicity as real))) *  (1.0 / (NumberOfPermutationsOf(xs[i+1..]) as real));
+       { assume {:axiom} false; }
+       (1.0 / ((length / multiplicity) as real)) *  (1.0 / (NumberOfPermutationsOf(xs[i+1..]) as real));
+       { assume {:axiom} false; assert 1.0 * 1.0 == 1.0; assert ((length / multiplicity) as real) * (NumberOfPermutationsOf(xs[i+1..]) as real) == (((length / multiplicity) * NumberOfPermutationsOf(xs[i+1..])) as real); }
+       1.0 / (((length / multiplicity) * NumberOfPermutationsOf(xs[i+1..])) as real);    
+       { assume {:axiom} false; assert xs[i+1..] == xs[i..][1..]; }        
+       1.0 / (((length / multiplicity) * NumberOfPermutationsOf(xs[i..][1..])) as real);  
+       { assume {:axiom} false; }      
+       1.0 / (NumberOfPermutationsOf(xs[i..]) as real);
+     } */
+     }
+   } */
 
-  lemma CorrectnessMultiset<T>(xs: seq<T>, x: T, i: nat := 0)
+  lemma {:axiom} CorrectnessMultiset<T>(xs: seq<T>, x: T, i: nat := 0)
     requires i <= |xs| - 1
     decreases |xs| - i
     ensures
@@ -138,117 +119,117 @@ module FisherYates.Correctness {
       var length := |xs[i..]|;
       && e in Rand.eventSpace
       && Rand.prob(e) == (multiplicity as real) / (length as real)
-  {
-    var A := iset j: int | i <= j < |xs| && xs[j] == x;
-    var e := Monad.BitstreamsWithValueIn(Uniform.Model.IntervalSample(i, |xs|), A);
-    var multiplicity := multiset(xs[i..])[x];
-    var length := |xs[i..]|;
-    if i == |xs| - 1 {
-      assert length == 1;
-      if xs[i] == x {
-        assert A == iset{ |xs| - 1 };
-        assert multiplicity == 1;
-        Uniform.Correctness.UniformFullIntervalCorrectness(i, |xs|, i);
-      } else {
-        assert A == iset{};
-        assert e == iset{};
-        assert multiplicity == 0;
-        Rand.ProbIsProbabilityMeasure();
-        assert Measures.IsPositive(Rand.eventSpace, Rand.prob);
-      }
-    } else {
-      var A' := iset j: int | i+1 <= j < |xs| && xs[j] == x;
-      var e' := Monad.BitstreamsWithValueIn(Uniform.Model.IntervalSample(i+1, |xs|), A');
-      assert e'Equality: e' == Monad.BitstreamsWithValueIn(Uniform.Model.IntervalSample(i, |xs|), A') by {
-        assume {:axiom} false;
-      }
-      var e'':= (iset s | Uniform.Model.IntervalSample(i, |xs|)(s).Equals(i as int));
-      var multiplicity' := multiset(xs[i+1..])[x];
-      var length' := |xs[i+1..]|;
-      assert InductionHypothesis: e' in Rand.eventSpace && Rand.prob(e') == (multiplicity' as real) / (length' as real) by {
-        CorrectnessMultiset(xs, x, i+1);
-      }
-      assert length == 1 + length';
-      if xs[i] == x {
-        assert multiplicity == 1 + multiplicity' by {
-          calc {
-            multiplicity;
-            multiset(xs[i..])[x];
-            { assert xs[i..] == [xs[i]] + xs[i+1..]; }
-            multiset([xs[i]] + xs[i+1..])[x];
-            (multiset([xs[i]]) + multiset(xs[i+1..]))[x];
-            multiset([xs[i]])[x] + multiset(xs[i+1..])[x];
-            1 + multiset(xs[i+1..])[x];
-            1 + multiplicity';
-          }
-        }
-        calc {
-          e;
-          Monad.BitstreamsWithValueIn(Uniform.Model.IntervalSample(i, |xs|), A);
-          { assert A == A' + iset{i as int}; }
-          Monad.BitstreamsWithValueIn(Uniform.Model.IntervalSample(i, |xs|), A' + iset{i as int});
-          { Monad.BitstreamsWithValueInJoin(Uniform.Model.IntervalSample(i, |xs|), A', iset{i as int}); }
-          Monad.BitstreamsWithValueIn(Uniform.Model.IntervalSample(i, |xs|), A') + Monad.BitstreamsWithValueIn(Uniform.Model.IntervalSample(i, |xs|), iset{i as int});
-          { assume {:axiom} false; }
-          Monad.BitstreamsWithValueIn(Uniform.Model.IntervalSample(i+1, |xs|), A') + (iset s | Uniform.Model.IntervalSample(i, |xs|)(s).Equals(i as int));
-          e' + e'';
-        }
-        assert e''inEventSpace: e'' in Rand.eventSpace by {
-          Uniform.Correctness.UniformFullIntervalCorrectness(i, |xs|, i);
-        }
-        assert MultProb: Rand.prob(e' + e'') == Rand.prob(e') + Rand.prob(e'') by {
-          assume {:axiom} e' * e'' == iset{};
-          reveal e''inEventSpace;
-          reveal InductionHypothesis;
-          Rand.ProbIsProbabilityMeasure();
-          Measures.MeasureOfDisjointUnionIsSum(Rand.eventSpace, Rand.prob, e', e'');
-        }
-        calc {
-          Rand.prob(e);
-          Rand.prob(e' + e'');
-          { reveal MultProb; }
-          Rand.prob(e') + Rand.prob(e'');
-          { reveal InductionHypothesis; Uniform.Correctness.UniformFullIntervalCorrectness(i, |xs|, i as int); }
-          ((multiplicity' as real) / (length' as real)) + (1.0 / (|xs| - i) as real);
-          ((multiplicity' as real) / (length' as real)) + 1.0 / length as real;
-          ((multiplicity' as real) / (length' as real)) + 1.0 / (1 + length') as real;
-          { assume {:axiom} false; }
-          ((1 + multiplicity') as real) / ((1 + length') as real);
-          (multiplicity as real) / (length as real);
-        }
-      } else {
-        assert multiplicity == multiplicity' by {
-          calc {
-            multiplicity;
-            multiset(xs[i..])[x];
-            { assert xs[i..] == [xs[i]] + xs[i+1..]; }
-            multiset([xs[i]] + xs[i+1..])[x];
-            (multiset([xs[i]]) + multiset(xs[i+1..]))[x];
-            multiset([xs[i]])[x] + multiset(xs[i+1..])[x];
-            multiset(xs[i+1..])[x];
-            multiplicity';
-          }
-        }
-        calc {
-          e;
-          Monad.BitstreamsWithValueIn(Uniform.Model.IntervalSample(i, |xs|), A);
-          { assert A == A'; }
-          Monad.BitstreamsWithValueIn(Uniform.Model.IntervalSample(i, |xs|), A');
-          { reveal e'Equality; }
-          e';
-        }
-        calc {
-          Rand.prob(e);
-          Rand.prob(e');
-          { reveal InductionHypothesis; }
-          (multiplicity' as real) / (length' as real);
-          { assume {:axiom} false; }
-          (multiplicity' as real) / ((1 + length') as real);
-          (multiplicity as real) / (length as real);
-        }
-      }
-    }
-  }
+  /*  {
+     var A := iset j: int | i <= j < |xs| && xs[j] == x;
+     var e := Monad.BitstreamsWithValueIn(Uniform.Model.IntervalSample(i, |xs|), A);
+     var multiplicity := multiset(xs[i..])[x];
+     var length := |xs[i..]|;
+     if i == |xs| - 1 {
+       assert length == 1;
+       if xs[i] == x {
+         assert A == iset{ |xs| - 1 };
+         assert multiplicity == 1;
+         Uniform.Correctness.UniformFullIntervalCorrectness(i, |xs|, i);
+       } else {
+         assert A == iset{};
+         assert e == iset{};
+         assert multiplicity == 0;
+         Rand.ProbIsProbabilityMeasure();
+         assert Measures.IsPositive(Rand.eventSpace, Rand.prob);
+       }
+     } else {
+       var A' := iset j: int | i+1 <= j < |xs| && xs[j] == x;
+       var e' := Monad.BitstreamsWithValueIn(Uniform.Model.IntervalSample(i+1, |xs|), A');
+       assert e'Equality: e' == Monad.BitstreamsWithValueIn(Uniform.Model.IntervalSample(i, |xs|), A') by {
+         assume {:axiom} false;
+       }
+       var e'':= (iset s | Uniform.Model.IntervalSample(i, |xs|)(s).Equals(i as int));
+       var multiplicity' := multiset(xs[i+1..])[x];
+       var length' := |xs[i+1..]|;
+       assert InductionHypothesis: e' in Rand.eventSpace && Rand.prob(e') == (multiplicity' as real) / (length' as real) by {
+         CorrectnessMultiset(xs, x, i+1);
+       }
+       assert length == 1 + length';
+       if xs[i] == x {
+         assert multiplicity == 1 + multiplicity' by {
+           calc {
+             multiplicity;
+             multiset(xs[i..])[x];
+             { assert xs[i..] == [xs[i]] + xs[i+1..]; }
+             multiset([xs[i]] + xs[i+1..])[x];
+             (multiset([xs[i]]) + multiset(xs[i+1..]))[x];
+             multiset([xs[i]])[x] + multiset(xs[i+1..])[x];
+             1 + multiset(xs[i+1..])[x];
+             1 + multiplicity';
+           }
+         }
+         calc {
+           e;
+           Monad.BitstreamsWithValueIn(Uniform.Model.IntervalSample(i, |xs|), A);
+           { assert A == A' + iset{i as int}; }
+           Monad.BitstreamsWithValueIn(Uniform.Model.IntervalSample(i, |xs|), A' + iset{i as int});
+           { Monad.BitstreamsWithValueInJoin(Uniform.Model.IntervalSample(i, |xs|), A', iset{i as int}); }
+           Monad.BitstreamsWithValueIn(Uniform.Model.IntervalSample(i, |xs|), A') + Monad.BitstreamsWithValueIn(Uniform.Model.IntervalSample(i, |xs|), iset{i as int});
+           { assume {:axiom} false; }
+           Monad.BitstreamsWithValueIn(Uniform.Model.IntervalSample(i+1, |xs|), A') + (iset s | Uniform.Model.IntervalSample(i, |xs|)(s).Equals(i as int));
+           e' + e'';
+         }
+         assert e''inEventSpace: e'' in Rand.eventSpace by {
+           Uniform.Correctness.UniformFullIntervalCorrectness(i, |xs|, i);
+         }
+         assert MultProb: Rand.prob(e' + e'') == Rand.prob(e') + Rand.prob(e'') by {
+           assume {:axiom} e' * e'' == iset{};
+           reveal e''inEventSpace;
+           reveal InductionHypothesis;
+           Rand.ProbIsProbabilityMeasure();
+           Measures.MeasureOfDisjointUnionIsSum(Rand.eventSpace, Rand.prob, e', e'');
+         }
+         calc {
+           Rand.prob(e);
+           Rand.prob(e' + e'');
+           { reveal MultProb; }
+           Rand.prob(e') + Rand.prob(e'');
+           { reveal InductionHypothesis; Uniform.Correctness.UniformFullIntervalCorrectness(i, |xs|, i as int); }
+           ((multiplicity' as real) / (length' as real)) + (1.0 / (|xs| - i) as real);
+           ((multiplicity' as real) / (length' as real)) + 1.0 / length as real;
+           ((multiplicity' as real) / (length' as real)) + 1.0 / (1 + length') as real;
+           { assume {:axiom} false; }
+           ((1 + multiplicity') as real) / ((1 + length') as real);
+           (multiplicity as real) / (length as real);
+         }
+       } else {
+         assert multiplicity == multiplicity' by {
+           calc {
+             multiplicity;
+             multiset(xs[i..])[x];
+             { assert xs[i..] == [xs[i]] + xs[i+1..]; }
+             multiset([xs[i]] + xs[i+1..])[x];
+             (multiset([xs[i]]) + multiset(xs[i+1..]))[x];
+             multiset([xs[i]])[x] + multiset(xs[i+1..])[x];
+             multiset(xs[i+1..])[x];
+             multiplicity';
+           }
+         }
+         calc {
+           e;
+           Monad.BitstreamsWithValueIn(Uniform.Model.IntervalSample(i, |xs|), A);
+           { assert A == A'; }
+           Monad.BitstreamsWithValueIn(Uniform.Model.IntervalSample(i, |xs|), A');
+           { reveal e'Equality; }
+           e';
+         }
+         calc {
+           Rand.prob(e);
+           Rand.prob(e');
+           { reveal InductionHypothesis; }
+           (multiplicity' as real) / (length' as real);
+           { assume {:axiom} false; }
+           (multiplicity' as real) / ((1 + length') as real);
+           (multiplicity as real) / (length as real);
+         }
+       }
+     }
+   } */
 
 
 
