src/Util/FisherYates/Model.dfy
@@ -7,6 +7,7 @@ module FisherYates.Model {
   import Monad
   import Uniform
   import Rand
+  import Permutations
 
   ghost function Shuffle<T>(xs: seq<T>, i: nat := 0): (h: Monad.Hurd<seq<T>>)
     requires i <= |xs|
@@ -17,21 +18,9 @@ module FisherYates.Model {
     (s: Rand.Bitstream) =>
       if |xs[i..]| > 1 then
         var (j, s) :- Uniform.Model.IntervalSample(i, |xs|)(s);
-        var xs := Swap(xs, i, j);
+        var xs := Permutations.Swap(xs, i, j);
         Shuffle(xs, i + 1)(s)
       else
         Monad.Return(xs)(s)
-  }
-
-  function Swap<T>(s: seq<T>, i: nat, j: nat): (t: seq<T>)
-    requires i <= j
-    requires 0 <= i < |s|
-    requires 0 <= j < |s|
-    ensures |s| == |t|
-  {
-    if i == j then
-      s
-    else
-      s[..i] + [s[j]] + s[i+1..j] + [s[i]] + s[j+1..]
   }
 }
